Add own erase dups function; resolve sorries

ProofLibrary/List.lean
@@ -335,6 +335,29 @@ namespace List
     | nil => contradiction
     | cons head tail => simp
 
+  def eraseDupsKeepRight [DecidableEq α] : List α -> List α
+  | [] => []
+  | hd::tl => if hd ∈ tl then tl.eraseDupsKeepRight else hd::(tl.eraseDupsKeepRight)
+
+  theorem mem_eraseDupsKeepRight_iff [DecidableEq α] (l : List α) : ∀ e, e ∈ l.eraseDupsKeepRight ↔ e ∈ l := by
+    induction l with
+    | nil => simp [eraseDupsKeepRight]
+    | cons hd tl ih =>
+      unfold eraseDupsKeepRight
+      intro e
+      cases Decidable.em (hd ∈ tl) with
+      | inl mem => simp [mem]; rw [ih]; simp; intro eq; rw [eq]; exact mem
+      | inr not_mem => simp [not_mem]; rw [ih]
+
+  theorem nodup_eraseDupsKeepRight [DecidableEq α] (l : List α) : l.eraseDupsKeepRight.Nodup := by
+    induction l with
+    | nil => simp [eraseDupsKeepRight]
+    | cons hd tl ih =>
+      simp only [eraseDupsKeepRight]
+      cases Decidable.em (hd ∈ tl) with
+      | inl mem => simp [mem, ih]
+      | inr not_mem => simp [not_mem, ih]; rw [mem_eraseDupsKeepRight_iff]; exact not_mem
+
 end List
 
 def List.repeat (val : α) : Nat -> List α
